pulse/lib/pulse/lib/Pulse.Lib.Slice.fsti
@@ -8,17 +8,17 @@ val slice : Type0 -> Type0
 
 val len (#t: Type) : slice t -> SZ.t
 
-val pts_to (#t: Type) (s: slice t) (#[exact (`1.0R)] p: perm) (v: Seq.seq t) : vprop
+val pts_to (#t: Type) (s: slice t) (#[exact (`1.0R)] p: perm) (v: Seq.seq t) : slprop
 
-val pts_to_is_small (#a:Type) (x:slice a) (p:perm) (s:Seq.seq a)
-  : Lemma (is_small (pts_to x #p s))
-          [SMTPat (is_small (pts_to x #p s))]
+val pts_to_is_slprop2 (#a:Type) (x:slice a) (p:perm) (s:Seq.seq a)
+  : Lemma (is_slprop2 (pts_to x #p s))
+          [SMTPat (is_slprop2 (pts_to x #p s))]
 
 val pts_to_len (#t: Type) (s: slice t) (#p: perm) (#v: Seq.seq t) : stt_ghost unit emp_inames
     (pts_to s #p v)
     (fun _ -> pts_to s #p v ** pure (Seq.length v == SZ.v (len s)))
 
-val is_from_array (#t: Type) (a: array t) (p: perm) (s: slice t) : vprop
+val is_from_array (#t: Type) (a: array t) (p: perm) (s: slice t) : slprop
 
 val from_array (#t: Type) (mutb: bool) (a: array t) (#p: perm) (#v: Ghost.erased (Seq.seq t)) (alen: SZ.t {
     SZ.v alen == A.length a /\
@@ -81,11 +81,11 @@ val gather
       (requires pts_to arr #p0 s0 ** pts_to arr #p1 s1)
       (ensures fun _ -> pts_to arr #(p0 +. p1) s0 ** pure (s0 == s1))
 
-val is_split (#t: Type) (s: slice t) (p: perm) (i: SZ.t) (left: slice t) (right: slice t) : vprop
+val is_split (#t: Type) (s: slice t) (p: perm) (i: SZ.t) (left: slice t) (right: slice t) : slprop
 
-val is_split_is_small (#t: Type) (s: slice t) (p: perm) (i: SZ.t) (left: slice t) (right: slice t)
-  : Lemma (is_small (is_split s p i left right))
-          [SMTPat (is_small (is_split s p i left right))]
+val is_split_is_slprop2 (#t: Type) (s: slice t) (p: perm) (i: SZ.t) (left: slice t) (right: slice t)
+  : Lemma (is_slprop2 (is_split s p i left right))
+          [SMTPat (is_slprop2 (is_split s p i left right))]
 
 noeq type slice_pair (t: Type) = | SlicePair: (fst: slice t) -> (snd: slice t) -> slice_pair t
 
@@ -98,7 +98,7 @@ let split_post'
     (#t: Type) (s: slice t) (p: perm) (v: Ghost.erased (Seq.seq t)) (i: SZ.t)
     (s1: slice t)
     (s2: slice t)
-: Tot vprop
+: Tot slprop
 =       exists* v1 v2 .
             pts_to s1 #p v1 **
             pts_to s2 #p v2 **
@@ -111,7 +111,7 @@ let split_post'
 let split_post
     (#t: Type) (s: slice t) (p: perm) (v: Ghost.erased (Seq.seq t)) (i: SZ.t)
     (res: slice_pair t)
-: Tot vprop
+: Tot slprop
 = let SlicePair s1 s2 = res in
     split_post' s p v i s1 s2
 
